code/rsapss/Hacl.Impl.RSAPSS.fst
@@ -11,265 +11,27 @@ open Hacl.Bignum.Definitions
 open Hacl.Bignum
 open Hacl.Bignum.Exponentiation
 
-open Hacl.Impl.MGF
-
 module ST = FStar.HyperStack.ST
-module LSeq = Lib.Sequence
-module HS = FStar.HyperStack
 
 module Hash = Spec.Agile.Hash
+module SB = Hacl.Spec.Bignum
+module BB = Hacl.Spec.Bignum.Base
+
 module S = Spec.RSAPSS
 module LS = Hacl.Spec.RSAPSS
-module SB = Hacl.Spec.Bignum
 
-#reset-options "--z3rlimit 50 --fuel 0 --ifuel 0"
-
-inline_for_extraction noextract
-let salt_len_t (a:Hash.algorithm) =
-  sLen:size_t{8 + Hash.hash_length a + v sLen <= max_size_t /\ 8 + Hash.hash_length a + v sLen <= Hash.max_input_length a}
-
-inline_for_extraction noextract
-let msg_len_t (a:Hash.algorithm) =
-  msgLen:size_t{v msgLen <= Hash.max_input_length a}
-
-inline_for_extraction noextract
-let em_len_t (a:Hash.algorithm) (sLen:salt_len_t a) =
-  emBits:size_t{0 < v emBits /\ Hash.hash_length a + v sLen + 2 <= v (blocks emBits 8ul)}
-
-inline_for_extraction noextract
-let pkey_len_pre (modBits:size_t) (eBits:size_t) =
-  1 < v modBits /\ 0 < v eBits /\
-  128 * v (blocks modBits 64ul) <= max_size_t /\
-  64 * v (blocks eBits 64ul) <= max_size_t /\
-  2 * v (blocks modBits 64ul) + v (blocks eBits 64ul) <= max_size_t
-
-inline_for_extraction noextract
-let skey_len_pre (modBits:size_t) (eBits:size_t) (dBits:size_t) =
-  pkey_len_pre modBits eBits /\
-  0 < v dBits /\ 64 * v (blocks dBits 64ul) <= max_size_t /\
-  2 * v (blocks modBits 64ul) + v (blocks eBits 64ul) + v (blocks dBits 64ul) <= max_size_t
+open Hacl.Impl.RSAPSS.Padding
+open Hacl.Impl.RSAPSS.MGF
 
 
-val xor_bytes:
-    len:size_t{v len > 0}
-  -> b1:lbuffer uint8 len
-  -> b2:lbuffer uint8 len ->
-  Stack unit
-  (requires fun h -> live h b1 /\ live h b2 /\ disjoint b1 b2)
-  (ensures  fun h0 _ h1 -> modifies (loc b1) h0 h1 /\
-    as_seq h1 b1 == S.xor_bytes (as_seq h0 b1) (as_seq h0 b2))
-
-[@CInline]
-let xor_bytes len b1 b2 =
-  map2T len b1 (fun x y -> x ^. y) b1 b2
-
-inline_for_extraction noextract
-val db_zero:
-    len:size_t{v len > 0}
-  -> db:lbuffer uint8 len
-  -> emBits:size_t ->
-  Stack unit
-  (requires fun h -> live h db)
-  (ensures  fun h0 _ h1 -> modifies (loc db) h0 h1 /\
-    as_seq h1 db == S.db_zero #(v len) (as_seq h0 db) (v emBits))
-
-let db_zero len db emBits =
-  let msBits = emBits %. 8ul in
-  if msBits >. 0ul then
-    db.(0ul) <- db.(0ul) &. (u8 0xff >>. (8ul -. msBits))
-
-
-inline_for_extraction noextract
-val get_m1Hash:
-    a:Hash.algorithm{S.hash_is_supported a}
-  -> sLen:salt_len_t a
-  -> salt:lbuffer uint8 sLen
-  -> msgLen:msg_len_t a
-  -> msg:lbuffer uint8 msgLen
-  -> hLen:size_t{v hLen == Hash.hash_length a}
-  -> m1Hash:lbuffer uint8 hLen ->
-  Stack unit
-  (requires fun h ->
-    live h salt /\ live h msg /\ live h m1Hash /\
-    disjoint msg salt /\ disjoint m1Hash msg /\ disjoint m1Hash salt)
-  (ensures  fun h0 _ h1 -> modifies (loc m1Hash) h0 h1 /\
-    (let mHash = Hash.hash a (as_seq h0 msg) in
-    let m1Len = 8 + Hash.hash_length a + v sLen in
-    let m1 = LSeq.create m1Len (u8 0) in
-    let m1 = LSeq.update_sub m1 8 (Hash.hash_length a) mHash in
-    let m1 = LSeq.update_sub m1 (8 + Hash.hash_length a) (v sLen) (as_seq h0 salt) in
-    as_seq h1 m1Hash == Hash.hash a m1))
-
-let get_m1Hash a sLen salt msgLen msg hLen m1Hash =
-  push_frame ();
-  //m1 = [8 * 0x00; mHash; salt]
-  let m1Len = 8ul +! hLen +! sLen in
-  let m1 = create m1Len (u8 0) in
-  let h0 = ST.get () in
-  update_sub_f h0 m1 8ul hLen
-    (fun h -> Hash.hash a (as_seq h0 msg))
-    (fun _ -> hash a (sub m1 8ul hLen) msgLen msg);
-  update_sub m1 (8ul +! hLen) sLen salt;
-  hash a m1Hash m1Len m1;
-  pop_frame()
-
-
-inline_for_extraction noextract
-val get_maskedDB:
-    a:Hash.algorithm{S.hash_is_supported a}
-  -> sLen:salt_len_t a
-  -> salt:lbuffer uint8 sLen
-  -> hLen:size_t{v hLen == Hash.hash_length a}
-  -> m1Hash:lbuffer uint8 hLen
-  -> emBits:em_len_t a sLen
-  -> dbLen:size_t{v dbLen == v (blocks emBits 8ul -! hash_len a -! 1ul)}
-  -> db_mask:lbuffer uint8 dbLen ->
-  Stack unit
-  (requires fun h ->
-    live h salt /\ live h m1Hash /\ live h db_mask /\
-    disjoint m1Hash salt /\ disjoint m1Hash db_mask /\ disjoint db_mask salt /\
-    as_seq h db_mask == LSeq.create (v dbLen) (u8 0))
-  (ensures  fun h0 _ h1 -> modifies (loc db_mask) h0 h1 /\
-   (let emLen = S.blocks (v emBits) 8 in
-    let dbLen = emLen - Hash.hash_length a - 1 in
-    let db = LSeq.create dbLen (u8 0) in
-    let last_before_salt = dbLen - v sLen - 1 in
-    let db = LSeq.upd db last_before_salt (u8 1) in
-    let db = LSeq.update_sub db (last_before_salt + 1) (v sLen) (as_seq h0 salt) in
-
-    let dbMask = S.mgf_hash a (v hLen) (as_seq h0 m1Hash) dbLen in
-    let maskedDB = S.xor_bytes db dbMask in
-    let maskedDB = S.db_zero maskedDB (v emBits) in
-    as_seq h1 db_mask == maskedDB))
-
-let get_maskedDB a sLen salt hLen m1Hash emBits dbLen db =
-  push_frame ();
-  //db = [0x00;..; 0x00; 0x01; salt]
-  let last_before_salt = dbLen -! sLen -! 1ul in
-  db.(last_before_salt) <- u8 1;
-  update_sub db (last_before_salt +! 1ul) sLen salt;
-
-  let dbMask = create dbLen (u8 0) in
-  assert_norm (Hash.hash_length a + 4 <= max_size_t /\ Hash.hash_length a + 4 <= Hash.max_input_length a);
-  mgf_hash a hLen m1Hash dbLen dbMask;
-  xor_bytes dbLen db dbMask;
-  db_zero dbLen db emBits;
-  pop_frame()
-
-
-val pss_encode:
-    a:Hash.algorithm{S.hash_is_supported a}
-  -> sLen:salt_len_t a
-  -> salt:lbuffer uint8 sLen
-  -> msgLen:msg_len_t a
-  -> msg:lbuffer uint8 msgLen
-  -> emBits:em_len_t a sLen
-  -> em:lbuffer uint8 (blocks emBits 8ul) ->
-  Stack unit
-  (requires fun h ->
-    live h salt /\ live h msg /\ live h em /\
-    disjoint msg salt /\ disjoint em msg /\ disjoint em salt /\
-    as_seq h em == LSeq.create (S.blocks (v emBits) 8) (u8 0))
-  (ensures  fun h0 _ h1 -> modifies (loc em) h0 h1 /\
-    as_seq h1 em == S.pss_encode a (v sLen) (as_seq h0 salt) (v msgLen) (as_seq h0 msg) (v emBits))
-
-[@CInline]
-let pss_encode a sLen salt msgLen msg emBits em =
-  push_frame ();
-  let hLen = hash_len a in
-  let m1Hash = create hLen (u8 0) in
-  get_m1Hash a sLen salt msgLen msg hLen m1Hash;
-
-  let emLen = blocks emBits 8ul in
-  let dbLen = emLen -! hLen -! 1ul in
-  let db = create dbLen (u8 0) in
-  get_maskedDB a sLen salt hLen m1Hash emBits dbLen db;
-
-  update_sub em 0ul dbLen db;
-  update_sub em dbLen hLen m1Hash;
-  em.(emLen -! 1ul) <- u8 0xbc;
-  pop_frame()
-
-
-inline_for_extraction noextract
-val pss_verify_:
-    a:Hash.algorithm{S.hash_is_supported a}
-  -> sLen:salt_len_t a
-  -> msgLen:msg_len_t a
-  -> msg:lbuffer uint8 msgLen
-  -> emBits:em_len_t a sLen
-  -> em:lbuffer uint8 (blocks emBits 8ul) ->
-  Stack bool
-  (requires fun h -> live h msg /\ live h em /\ disjoint em msg)
-  (ensures  fun h0 r h1 -> modifies0 h0 h1 /\
-    r == S.pss_verify_ a (v sLen) (v msgLen) (as_seq h0 msg) (v emBits) (as_seq h0 em))
-
-let pss_verify_ a sLen msgLen msg emBits em =
-  push_frame ();
-  let emLen = blocks emBits 8ul in
-
-  let hLen = hash_len a in
-  let m1Hash0 = create hLen (u8 0) in
-  let dbLen = emLen -! hLen -! 1ul in
-  let maskedDB = sub em 0ul dbLen in
-  let m1Hash = sub em dbLen hLen in
-
-  let dbMask = create dbLen (u8 0) in
-  mgf_hash a hLen m1Hash dbLen dbMask;
-  xor_bytes dbLen dbMask maskedDB;
-  db_zero dbLen dbMask emBits;
-
-  let padLen = emLen -! sLen -! hLen -! 1ul in
-  let pad2 = create padLen (u8 0) in
-  pad2.(padLen -! 1ul) <- u8 0x01;
-
-  let pad = sub dbMask 0ul padLen in
-  let salt = sub dbMask padLen sLen in
-
-  let res =
-    if not (Lib.ByteBuffer.lbytes_eq #padLen pad pad2) then false
-    else begin
-      get_m1Hash a sLen salt msgLen msg hLen m1Hash0;
-      Lib.ByteBuffer.lbytes_eq #hLen m1Hash0 m1Hash end in
-  pop_frame ();
-  res
-
-
-#set-options "--z3rlimit 300"
-
-val pss_verify:
-    a:Hash.algorithm{S.hash_is_supported a}
-  -> sLen:salt_len_t a
-  -> msgLen:msg_len_t a
-  -> msg:lbuffer uint8 msgLen
-  -> emBits:size_t{0 < v emBits}
-  -> em:lbuffer uint8 (blocks emBits 8ul) ->
-  Stack bool
-  (requires fun h -> live h msg /\ live h em /\ disjoint em msg)
-  (ensures  fun h0 r h1 -> modifies0 h0 h1 /\
-    r == S.pss_verify a (v sLen) (v msgLen) (as_seq h0 msg) (v emBits) (as_seq h0 em))
-
-[@CInline]
-let pss_verify a sLen msgLen msg emBits em =
-  let emLen = blocks emBits 8ul in
-  let msBits = emBits %. 8ul in
-
-  let em_0 = if msBits >. 0ul then em.(0ul) &. (u8 0xff <<. msBits) else u8 0 in
-  let em_last = em.(emLen -! 1ul) in
-
-  if (emLen <. sLen +! hash_len a +! 2ul) then false
-  else begin
-    if not (FStar.UInt8.(Lib.RawIntTypes.u8_to_UInt8 em_last =^ 0xbcuy) &&
-      FStar.UInt8.(Lib.RawIntTypes.u8_to_UInt8 em_0 =^ 0uy)) then false
-    else pss_verify_ a sLen msgLen msg emBits em end
-
+#reset-options "--z3rlimit 150 --fuel 0 --ifuel 0"
 
 inline_for_extraction noextract
 val rsapss_sign_:
     a:Hash.algorithm{S.hash_is_supported a}
   -> modBits:size_t
   -> eBits:size_t
-  -> dBits:size_t{skey_len_pre modBits eBits dBits}
+  -> dBits:size_t{LS.skey_len_pre (v modBits) (v eBits) (v dBits)}
   -> skey:lbignum (2ul *! blocks modBits 64ul +! blocks eBits 64ul +! blocks dBits 64ul)
   -> sLen:size_t
   -> salt:lbuffer uint8 sLen
@@ -284,18 +46,9 @@ val rsapss_sign_:
 
     LS.rsapss_sign_pre a (v modBits) (v eBits) (v dBits) (as_seq h skey)
       (v sLen) (as_seq h salt) (v msgLen) (as_seq h msg))
-  (ensures  fun h0 b h1 -> modifies (loc sgnt) h0 h1 /\
-   (let nLen = blocks modBits 64ul in
-    let eLen = blocks eBits 64ul in
-    let dLen = blocks dBits 64ul in
-
-    let n = bn_v h0 (gsub skey 0ul nLen) in
-    let e = bn_v h0 (gsub skey (nLen +! nLen) eLen) in
-    let d = bn_v h0 (gsub skey (nLen +! nLen +! eLen) dLen) in
-    let pkeys : S.rsa_pubkey (v modBits) = S.Mk_rsa_pubkey n e in
-    let skeys : S.rsa_privkey (v modBits) = S.Mk_rsa_privkey pkeys d in
-    let sgnt_s = S.rsapss_sign_ a (v modBits) skeys (v sLen) (as_seq h0 salt) (v msgLen) (as_seq h0 msg) in
-    if b then Some? sgnt_s /\ as_seq h1 sgnt == Some?.v sgnt_s else None? sgnt_s))
+  (ensures  fun h0 eq_m h1 -> modifies (loc sgnt) h0 h1 /\
+    LS.rsapss_sign_post a (v modBits) (v eBits) (v dBits) (as_seq h0 skey)
+      (v sLen) (as_seq h0 salt) (v msgLen) (as_seq h0 msg) eq_m (as_seq h1 sgnt))
 
 let rsapss_sign_ a modBits eBits dBits skey sLen salt msgLen msg sgnt =
   push_frame ();
@@ -331,8 +84,6 @@ let rsapss_sign_ a modBits eBits dBits skey sLen salt msgLen msg sgnt =
   let _ = bn_mod_exp_precompr2 nLen n s eBits e r2 m' in
 
   let eq_m = bn_eq_mask nLen m m' in
-  let h_m = ST.get () in
-  Hacl.Spec.Bignum.bn_eq_mask_lemma (as_seq h_m m) (as_seq h_m m');
   mapT nLen s (logand eq_m) s;
 
   LS.blocks_bits_lemma (v modBits);
@@ -340,12 +91,10 @@ let rsapss_sign_ a modBits eBits dBits skey sLen salt msgLen msg sgnt =
   bn_to_bytes_be k s sgnt;
 
   let h_final = ST.get () in
-  //assert (as_seq h_final sgnt == LS.rsapss_sign a (v modBits) (v eBits) (v dBits)
-  //(as_seq h_init skey) (v sLen) (as_seq h_init salt) (v msgLen) (as_seq h_init msg));
   LS.rsapss_sign_lemma a (v modBits) (v eBits) (v dBits)
     (as_seq h_init skey) (v sLen) (as_seq h_init salt) (v msgLen) (as_seq h_init msg);
   pop_frame ();
-  Hacl.Bignum.Base.unsafe_bool_of_u64 eq_m
+  BB.unsafe_bool_of_u64 eq_m
 
 
 inline_for_extraction noextract
@@ -374,8 +123,8 @@ let rsapss_sign_st (a:Hash.algorithm{S.hash_is_supported a}) =
     let n = bn_v h0 (gsub skey 0ul nLen) in
     let e = bn_v h0 (gsub skey (nLen +! nLen) eLen) in
     let d = bn_v h0 (gsub skey (nLen +! nLen +! eLen) dLen) in
-    let pkeys : S.rsa_pubkey (v modBits) = S.Mk_rsa_pubkey n e in
-    let skeys : S.rsa_privkey (v modBits) = S.Mk_rsa_privkey pkeys d in
+    let pkeys : S.rsapss_pkey (v modBits) = S.Mk_rsapss_pkey n e in
+    let skeys : S.rsapss_skey (v modBits) = S.Mk_rsapss_skey pkeys d in
     let sgnt_s = S.rsapss_sign a (v modBits) skeys (v sLen) (as_seq h0 salt) (v msgLen) (as_seq h0 msg) in
     if b then Some? sgnt_s /\ as_seq h1 sgnt == Some?.v sgnt_s else None? sgnt_s))
 
@@ -394,7 +143,8 @@ let rsapss_sign a modBits eBits dBits skey sLen salt msgLen msg sgnt =
 
   if b then
     rsapss_sign_ a modBits eBits dBits skey sLen salt msgLen msg sgnt
-  else false
+  else
+    false
 
 
 
@@ -459,11 +209,11 @@ let rsapss_verify_ a modBits eBits pkey sLen sgnt msgLen msg =
 
   let mask = bn_lt_mask nLen s n in
   let res =
-    if FStar.UInt64.(Lib.RawIntTypes.u64_to_UInt64 mask =^ ones U64 PUB) then begin
+    if BB.unsafe_bool_of_u64 mask then begin
       let _ = bn_mod_exp_precompr2 nLen n s eBits e r2 m in
-
       LS.em_blocks_lt_max_size_t (v modBits);
       assert (8 * v (blocks emLen 8ul) <= max_size_t);
+
       if bn_lt_pow2 modBits m then begin
 	let m1 = sub m 0ul (blocks emLen 8ul) in
 	bn_to_bytes_be emLen m1 em;
@@ -471,8 +221,8 @@ let rsapss_verify_ a modBits eBits pkey sLen sgnt msgLen msg =
       else false end
     else false in
   pop_frame ();
-  assert (res == LS.rsapss_verify_ a (v modBits) (v eBits) (as_seq h_init pkey)
-    (v sLen) (as_seq h_init sgnt) (v msgLen) (as_seq h_init msg));
+  //assert (res == LS.rsapss_verify_ a (v modBits) (v eBits) (as_seq h_init pkey)
+    //(v sLen) (as_seq h_init sgnt) (v msgLen) (as_seq h_init msg));
   LS.rsapss_verify_lemma a (v modBits) (v eBits) (as_seq h_init pkey)
     (v sLen) (as_seq h_init sgnt) (v msgLen) (as_seq h_init msg);
   res
@@ -500,7 +250,7 @@ let rsapss_verify_st (a:Hash.algorithm{S.hash_is_supported a}) =
 
     let n = bn_v h0 (gsub pkey 0ul nLen) in
     let e = bn_v h0 (gsub pkey (nLen +! nLen) eLen) in
-    let pkeys : S.rsa_pubkey (v modBits) = S.Mk_rsa_pubkey n e in
+    let pkeys : S.rsapss_pkey (v modBits) = S.Mk_rsapss_pkey n e in
     r == S.rsapss_verify a (v modBits) pkeys (v sLen) (v k) (as_seq h0 sgnt) (v msgLen) (as_seq h0 msg)))
 
 
