code/rsapss/Hacl.Spec.RSAPSS.fst
@@ -10,6 +10,7 @@ open Hacl.Spec.Bignum
 open Hacl.Spec.Bignum.Exponentiation
 
 module S = Spec.RSAPSS
+module BB = Hacl.Spec.Bignum.Base
 module SM = Hacl.Spec.Bignum.Montgomery
 module BSeq = Lib.ByteSequence
 module Hash = Spec.Agile.Hash
@@ -162,8 +163,10 @@ val rsapss_sign_pre:
   -> msg:seq uint8{length msg == msgLen} -> Type0
 
 let rsapss_sign_pre a modBits eBits dBits skey sLen salt msgLen msg =
-  sLen + Hash.hash_length a + 8 <= max_size_t /\ sLen + Hash.hash_length a + 8 <= Hash.max_input_length a /\
-  sLen + Hash.hash_length a + 2 <= (blocks (modBits - 1) 8) /\ msgLen <= Hash.max_input_length a /\
+  sLen + Hash.hash_length a + 8 <= max_size_t /\
+  sLen + Hash.hash_length a + 8 <= Hash.max_input_length a /\
+  sLen + Hash.hash_length a + 2 <= (blocks (modBits - 1) 8) /\
+  msgLen <= Hash.max_input_length a /\
 
   rsapss_skey_pre modBits eBits dBits skey
 
@@ -178,9 +181,10 @@ val rsapss_sign_post:
   -> salt:lseq uint8 sLen
   -> msgLen:nat
   -> msg:seq uint8{length msg == msgLen}
-  -> sgnt:option (lseq uint8 (blocks modBits 8)) -> Type0
+  -> eq_m:bool
+  -> sgnt:lseq uint8 (blocks modBits 8) -> Type0
 
-let rsapss_sign_post a modBits eBits dBits skey sLen salt msgLen msg sgnt =
+let rsapss_sign_post a modBits eBits dBits skey sLen salt msgLen msg eq_m sgnt =
   rsapss_sign_pre a modBits eBits dBits skey sLen salt msgLen msg /\
  (let nLen = blocks modBits 64 in
   let eLen = blocks eBits 64 in
@@ -189,9 +193,10 @@ let rsapss_sign_post a modBits eBits dBits skey sLen salt msgLen msg sgnt =
   let n = bn_v (sub skey 0 nLen) in
   let e = bn_v (sub skey (nLen + nLen) eLen) in
   let d = bn_v (sub skey (nLen + nLen + eLen) dLen) in
-  let pkeys : S.rsa_pubkey modBits = S.Mk_rsa_pubkey n e in
-  let skeys : S.rsa_privkey modBits = S.Mk_rsa_privkey pkeys d in
-  sgnt == S.rsapss_sign_ a modBits skeys sLen salt msgLen msg)
+  let pkeys : S.rsapss_pkey modBits = S.Mk_rsapss_pkey n e in
+  let skeys : S.rsapss_skey modBits = S.Mk_rsapss_skey pkeys d in
+  let eq_m_s, sgnt_s = S.rsapss_sign_ a modBits skeys sLen salt msgLen msg in
+  eq_m_s == eq_m /\ (eq_m ==> sgnt == sgnt_s))
 
 
 val rsapss_verify_pre:
@@ -204,7 +209,8 @@ val rsapss_verify_pre:
   -> msg:seq uint8{length msg == msgLen} -> Type0
 
 let rsapss_verify_pre a modBits eBits pkey sLen msgLen msg =
-  sLen + Hash.hash_length a + 8 <= max_size_t /\ sLen + Hash.hash_length a + 8 <= Hash.max_input_length a /\
+  sLen + Hash.hash_length a + 8 <= max_size_t /\
+  sLen + Hash.hash_length a + 8 <= Hash.max_input_length a /\
   msgLen <= Hash.max_input_length a /\
 
   rsapss_pkey_pre modBits eBits pkey
@@ -228,7 +234,7 @@ let rsapss_verify_post a modBits eBits pkey sLen sgnt msgLen msg verify =
 
   let n = bn_v (sub pkey 0 nLen) in
   let e = bn_v (sub pkey (nLen + nLen) eLen) in
-  let pkeys : S.rsa_pubkey modBits = S.Mk_rsa_pubkey n e in
+  let pkeys : S.rsapss_pkey modBits = S.Mk_rsapss_pkey n e in
   verify == S.rsapss_verify_ a modBits pkeys sLen sgnt msgLen msg)
 
 
@@ -243,7 +249,7 @@ val rsapss_sign_:
   -> salt:lseq uint8 sLen
   -> msgLen:nat
   -> msg:seq uint8{length msg == msgLen}
-  -> Pure (option (lseq uint8 (blocks modBits 8)))
+  -> Pure (tuple2 bool (lseq uint8 (blocks modBits 8)))
   (requires rsapss_sign_pre a modBits eBits dBits skey sLen salt msgLen msg)
   (ensures  fun sgnt -> True)
 
@@ -276,8 +282,7 @@ let rsapss_sign_ a modBits eBits dBits skey sLen salt msgLen msg =
   blocks_bits_lemma modBits;
   assert (blocks k 8 == nLen);
   let sgnt = bn_to_bytes_be k s in
-
-  if Lib.RawIntTypes.u64_to_UInt64 eq_m = 0uL then None else Some sgnt
+  BB.unsafe_bool_of_u64 eq_m, sgnt
 
 
 val rsapss_sign_lemma:
@@ -293,8 +298,8 @@ val rsapss_sign_lemma:
   (requires
     rsapss_sign_pre a modBits eBits dBits skey sLen salt msgLen msg)
   (ensures
-    rsapss_sign_post a modBits eBits dBits skey sLen salt msgLen msg
-    (rsapss_sign_ a modBits eBits dBits skey sLen salt msgLen msg))
+   (let eq_m, s = rsapss_sign_ a modBits eBits dBits skey sLen salt msgLen msg in
+    rsapss_sign_post a modBits eBits dBits skey sLen salt msgLen msg eq_m s))
 
 let rsapss_sign_lemma a modBits eBits dBits skey sLen salt msgLen msg =
   let nLen = blocks modBits 64 in
@@ -330,8 +335,10 @@ let rsapss_sign_lemma a modBits eBits dBits skey sLen salt msgLen msg =
 
   let m' = bn_mod_exp_precompr2 nLen n s eBits e r2 in
   bn_mod_exp_precompr2_lemma nLen n s eBits e r2;
+
   let eq_m = bn_eq_mask m m' in
   bn_eq_mask_lemma m m';
+
   let s' = map (logand eq_m) s in
   bn_mask_lemma s eq_m;
 
@@ -373,7 +380,7 @@ let rsapss_verify_ a modBits eBits pkey sLen sgnt msgLen msg =
   let s = bn_from_bytes_be k sgnt in
 
   let mask = bn_lt_mask s n in
-  if FStar.UInt64.(Lib.RawIntTypes.u64_to_UInt64 mask =^ ones U64 PUB) then begin
+  if BB.unsafe_bool_of_u64 mask then begin
     let m = bn_mod_exp_precompr2 nLen n s eBits e r2 in
     em_blocks_lt_max_size_t modBits;
     assert (8 * blocks emLen 8 <= max_size_t);
@@ -423,7 +430,7 @@ let rsapss_verify_lemma a modBits eBits pkey sLen sgnt msgLen msg =
   bn_lt_mask_lemma s n;
 
   let res =
-  if FStar.UInt64.(Lib.RawIntTypes.u64_to_UInt64 mask =^ ones U64 PUB) then begin
+  if BB.unsafe_bool_of_u64 mask then begin
     let m = bn_mod_exp_precompr2 nLen n s eBits e r2 in
     Math.Lemmas.pow2_le_compat (64 * nLen) modBits;
     SM.precomp_r2_mod_n_lemma n;
@@ -443,3 +450,203 @@ let rsapss_verify_lemma a modBits eBits pkey sLen sgnt msgLen msg =
     else false in
     () end in
   ()
+
+
+
+val bn_check_num_bits: bits:size_pos -> b:lbignum (blocks bits 64) ->
+  res:uint64{v res == (if bn_v b < pow2 bits then v (ones U64 SEC) else v (zeros U64 SEC))}
+
+let bn_check_num_bits bits b =
+  let bLen = blocks bits 64 in
+  assert (bits <= 64 * bLen);
+  let m : uint64 = if bits = 64 * bLen then ones U64 SEC else bn_lt_pow2_mask b bits in
+  (if bits = 64 * bLen then begin
+    bn_eval_bound b bLen;
+    Math.Lemmas.pow2_le_compat (64 * bLen) bits end
+  else
+    bn_lt_pow2_mask_lemma b bits);
+  assert (v m == (if bn_v b < pow2 bits then v (ones U64 SEC) else v (zeros U64 SEC)));
+  m
+
+
+val rsapss_check_modulus: modBits:size_pos -> n:lbignum (blocks modBits 64) ->
+  res:uint64{v res == (if (bn_v n % 2 = 1 && pow2 (modBits - 1) < bn_v n && bn_v n < pow2 modBits) then v (ones U64 SEC) else v (zeros U64 SEC))}
+
+let rsapss_check_modulus modBits n =
+  let bit0 = bn_is_odd n in
+  bn_is_odd_lemma n;
+  assert (v bit0 == bn_v n % 2);
+  let m0 = u64 0 -. bit0 in
+
+  let m1 = bn_gt_pow2_mask n (modBits - 1) in
+  bn_gt_pow2_mask_lemma n (modBits - 1);
+
+  let m2 = bn_check_num_bits modBits n in
+  let m = m0 &. (m1 &. m2) in
+  logand_lemma m0 (m1 &. m2);
+  logand_lemma m1 m2;
+  m
+
+
+val rsapss_check_exponent: eBits:size_pos -> e:lbignum (blocks eBits 64) ->
+  res:uint64{v res == (if (0 < bn_v e && bn_v e < pow2 eBits) then v (ones U64 SEC) else v (zeros U64 SEC))}
+
+let rsapss_check_exponent eBits e =
+  let m0 = bn_is_zero_mask e in
+  bn_is_zero_mask_lemma e;
+  let m1 = bn_check_num_bits eBits e in
+  let m = (lognot m0) &. m1 in
+  lognot_lemma m0;
+  logand_lemma (lognot m0) m1;
+  m
+
+
+val rsapss_load_pkey_post:
+    modBits:size_nat
+  -> eBits:size_nat{pkey_len_pre modBits eBits}
+  -> nb:lseq uint8 (blocks modBits 8)
+  -> eb:lseq uint8 (blocks eBits 8)
+  -> pkey:lbignum (2 * blocks modBits 64 + blocks eBits 64) -> Type0
+
+let rsapss_load_pkey_post modBits eBits nb eb pkey =
+  let pkey_s = S.rsapss_load_pkey modBits eBits nb eb in
+
+  let nLen = blocks modBits 64 in
+  let eLen = blocks eBits 64 in
+
+  let n  = sub pkey 0 nLen in
+  let e  = sub pkey (nLen + nLen) eLen in
+
+  rsapss_pkey_pre modBits eBits pkey /\
+  Some? pkey_s /\
+  bn_v n == S.Mk_rsapss_pkey?.n (Some?.v pkey_s) /\
+  bn_v e == S.Mk_rsapss_pkey?.e (Some?.v pkey_s)
+
+
+
+val rsapss_load_skey_post:
+    modBits:size_nat
+  -> eBits:size_nat
+  -> dBits:size_nat{skey_len_pre modBits eBits dBits}
+  -> nb:lseq uint8 (blocks modBits 8)
+  -> eb:lseq uint8 (blocks eBits 8)
+  -> db:lseq uint8 (blocks dBits 8)
+  -> skey:lbignum (2 * blocks modBits 64 + blocks eBits 64 + blocks dBits 64) -> Type0
+
+let rsapss_load_skey_post modBits eBits dBits nb eb db skey =
+  let skey_s = S.rsapss_load_skey modBits eBits dBits nb eb db in
+
+  let nLen = blocks modBits 64 in
+  let eLen = blocks eBits 64 in
+  let dLen = blocks dBits 64 in
+
+  let n  = sub skey 0 nLen in
+  let e  = sub skey (nLen + nLen) eLen in
+  let d  = sub skey (nLen + nLen + eLen) dLen in
+
+  rsapss_skey_pre modBits eBits dBits skey /\
+  Some? skey_s /\ (let pkey_s = S.Mk_rsapss_skey?.pkey (Some?.v skey_s) in
+  bn_v n == S.Mk_rsapss_pkey?.n pkey_s /\
+  bn_v e == S.Mk_rsapss_pkey?.e pkey_s /\
+  bn_v d == S.Mk_rsapss_skey?.d (Some?.v skey_s))
+
+
+val rsapss_load_pkey:
+    modBits:size_nat
+  -> eBits:size_nat{pkey_len_pre modBits eBits}
+  -> nb:lseq uint8 (blocks modBits 8)
+  -> eb:lseq uint8 (blocks eBits 8) ->
+  tuple2 bool (lbignum (2 * blocks modBits 64 + blocks eBits 64))
+
+let rsapss_load_pkey modBits eBits nb eb =
+  let n  = bn_from_bytes_be (blocks modBits 8) nb in
+  let r2 = SM.precomp_r2_mod_n n in
+  let e  = bn_from_bytes_be (blocks eBits 8) eb in
+  let pkey = (n @| r2) @| e in
+
+  let m0 = rsapss_check_modulus modBits n in
+  let m1 = rsapss_check_exponent eBits e in
+  let m = m0 &. m1 in
+  BB.unsafe_bool_of_u64 m, pkey
+
+
+val rsapss_load_pkey_lemma:
+    modBits:size_nat
+  -> eBits:size_nat{pkey_len_pre modBits eBits}
+  -> nb:lseq uint8 (blocks modBits 8)
+  -> eb:lseq uint8 (blocks eBits 8) ->
+  Lemma (let b, pkey = rsapss_load_pkey modBits eBits nb eb in
+   (b ==> rsapss_load_pkey_post modBits eBits nb eb pkey))
+
+let rsapss_load_pkey_lemma modBits eBits nb eb =
+  let nbLen = blocks modBits 8 in
+  let ebLen = blocks eBits 8 in
+
+  let nLen = blocks modBits 64 in
+  let eLen = blocks eBits 64 in
+
+  let n  = bn_from_bytes_be nbLen nb in
+  bn_from_bytes_be_lemma nbLen nb;
+  let r2 = SM.precomp_r2_mod_n n in
+  let e  = bn_from_bytes_be ebLen eb in
+  bn_from_bytes_be_lemma ebLen eb;
+
+  let pkey = (n @| r2) @| e in
+  eq_intro (sub pkey 0 nLen) n;
+  eq_intro (sub pkey nLen nLen) r2;
+  eq_intro (sub pkey (nLen + nLen) eLen) e;
+
+
+  let m0 = rsapss_check_modulus modBits n in
+  let m1 = rsapss_check_exponent eBits e in
+  let m = m0 &. m1 in
+  logand_lemma m0 m1
+
+
+val rsapss_load_skey:
+    modBits:size_nat
+  -> eBits:size_nat
+  -> dBits:size_nat{skey_len_pre modBits eBits dBits}
+  -> nb:lseq uint8 (blocks modBits 8)
+  -> eb:lseq uint8 (blocks eBits 8)
+  -> db:lseq uint8 (blocks dBits 8) ->
+  tuple2 bool (lbignum (2 * blocks modBits 64 + blocks eBits 64 + blocks dBits 64))
+
+let rsapss_load_skey modBits eBits dBits nb eb db =
+  let b, pkey = rsapss_load_pkey modBits eBits nb eb in
+  let d = bn_from_bytes_be (blocks dBits 8) db in
+  let skey = pkey @| d in
+
+  let m0 = rsapss_check_exponent dBits d in
+  let b1 = b && BB.unsafe_bool_of_u64 m0 in
+  b1, skey
+
+
+val rsapss_load_skey_lemma:
+    modBits:size_nat
+  -> eBits:size_nat
+  -> dBits:size_nat{skey_len_pre modBits eBits dBits}
+  -> nb:lseq uint8 (blocks modBits 8)
+  -> eb:lseq uint8 (blocks eBits 8)
+  -> db:lseq uint8 (blocks dBits 8) ->
+  Lemma (let b, skey = rsapss_load_skey modBits eBits dBits nb eb db in
+   (b ==> rsapss_load_skey_post modBits eBits dBits nb eb db skey))
+
+let rsapss_load_skey_lemma modBits eBits dBits nb eb db =
+  let nbLen = blocks modBits 8 in
+  let ebLen = blocks eBits 8 in
+  let dbLen = blocks dBits 8 in
+
+  let nLen = blocks modBits 64 in
+  let eLen = blocks eBits 64 in
+  let dLen = blocks dBits 64 in
+
+  let b, pkey = rsapss_load_pkey modBits eBits nb eb in
+  rsapss_load_pkey_lemma modBits eBits nb eb;
+
+  let d = bn_from_bytes_be (blocks dBits 8) db in
+  bn_from_bytes_be_lemma (blocks dBits 8) db;
+
+  let skey = pkey @| d in
+  eq_intro (sub skey 0 (nLen + nLen + eLen)) pkey;
+  eq_intro (sub skey (nLen + nLen + eLen) dLen) d
